Add more syntatic sugar

shift-reset/interpreter/builtin.v
@@ -1,5 +1,6 @@
 From Stdlib Require Import List String ZArith.
 From shift_reset.lib Require list.
+From shift_reset.lib Require Import int.
 From shift_reset.core Require Import syntax tag.
 From shift_reset.interpreter Require Import ierror imonad unwrap.
 Import ListNotations.
@@ -7,12 +8,17 @@ Import ListNotations.
 Local Open Scope string_scope.
 Local Open Scope imonad_scope.
 
-Definition builtin_string_length (v : val) : imonad val :=
+Definition string_length (v : val) : imonad val :=
   s <- unwrap_vstring v;
   imonad_pure (VInt (Z.of_nat (String.length s))).
 
+Definition int_to_string (v : val) : imonad val :=
+  z <- unwrap_vint v;
+  imonad_pure (VString (Z_to_string z)).
+
 Definition builtin_registry : list (tag * (val -> imonad val)) :=
-  [(Tag "string_length", builtin_string_length)].
+  [(Tag "string_length", string_length);
+   (Tag "int_to_string", int_to_string)].
 
 Definition dispatch_builtin (tag : tag) : imonad (val -> imonad val) :=
   match list.lookup tag_eqb tag builtin_registry with
