shift-reset/core/syntax_notation.v
@@ -443,3 +443,9 @@ Notation "}" := TRecordNil (in custom record_term at level 23) : term_scope.
 
 Notation "t .( tag )" :=
   (TVProj t tag) (in custom term at level 23, tag constr at level 0) : term_scope.
+
+Notation "t1 .[ t2 ]" :=
+  (TVGetAt t1 t2) (in custom term at level 65, t1 custom term, t2 custom term) : term_scope.
+
+Notation "t1 ++ t2" :=
+  (Op2App t1 t2) (in custom term at level 49, t1 custom term, t2 custom term, right associativity) : term_scope.
