shift-reset/interpreter/ierror.v
@@ -9,6 +9,7 @@ Inductive ierror : Type :=
 | Memory_error : string -> ierror
 | Assert_failure : string -> ierror
 | Match_failure : string -> ierror
+| Invalid_argument : string -> ierror
 | Undelimited_shift : string -> ierror
 | Undelimited_control : string -> ierror
 | Unhandled_exception : string -> ierror
