shift-reset/lib/int.v
@@ -1,5 +1,7 @@
-From Stdlib Require Import ZArith.
+From Stdlib Require Import DecimalString String ZArith.
+Import NilZero.
 
 Local Open Scope Z_scope.
 
 Definition Z_neqb (z1 z2 : Z) : bool := negb (z1 =? z2).
+Definition Z_to_string (z : Z) : string := string_of_int (Z.to_int z).
